feat: proved helper theorems and partially proved determinism

OperationalSemantics/BigStep.lean
@@ -1,13 +1,12 @@
 import OperationalSemantics.Basic
 
-namespace WHILE
+namespace WHILELang
 
 inductive BigStep : (Program × State) → State → Prop where
   | skip {s : State} : BigStep (⟪ skip ⟫, s) s
-  | assignment {s : State} {v : Var} {e : Expr}
+  | assignment {s : State} (v : Var) (e : Expr)
     (he : ∃ w : Value, Option.some w = ⟦ e; s ⟧)
-    : BigStep ((Program.assignment v e), s)
-    (fun x => if x = v then Exists.choose e' else s x)
+    : BigStep ((Program.assignment v e), s) (s.sub v (Exists.choose he))
   | seq {s t u : State} {p₀ p₁ : Program}
     (hp₀ : BigStep (p₀, s) t)
     (hp₁ : BigStep (p₁, t) u)
@@ -23,17 +22,145 @@ inductive BigStep : (Program × State) → State → Prop where
   | while_true {s t u : State} {e : Expr} {p : Program}
     (htrue : ⟦ e; s ⟧ = Option.some (Value.bool true))
     (hp : BigStep (p, s) t)
-    (hwhile : BigStep ((Program.while e p), t) u)
-    : BigStep ((Program.while e p), s) u
+    (hwhile : BigStep ((Program.while_do e p), t) u)
+    : BigStep ((Program.while_do e p), s) u
   | while_false {s : State} {e : Expr} {p : Program}
     (hfalse : ⟦ e; s ⟧ = Option.some (Value.bool false))
-    : BigStep ((Program.while e p), s) s
+    : BigStep ((Program.while_do e p), s) s
 
 infixl:60 " ▷ " => BigStep
 
-theorem skip_state_invariant (s : State) : (⟪ skip ⟫, s) ▷ s := by constructor
+theorem skip_state_invariant (s : State) : (⟪ skip ⟫, s) ▷ s := by
+  exact @BigStep.skip s
 
-example : (⟪ skip ⟫, {x ← 2, y ← 2}) ▷ {y ← 2, x ← 2} := by
-  apply skip_state_invariant
+@[grind =]
+theorem big_step_skip_iff (s t : State) : (⟪ skip ⟫, s) ▷ t ↔ s = t := by
+  constructor
+  · intro h
+    cases h; rfl
+  · intro h
+    rw [h]
+    apply skip_state_invariant
 
-end WHILE
+@[grind =]
+theorem big_step_assignment_iff (s t : State) (v : Var) (e : Expr) : (Program.assignment v e, s) ▷ t ↔ ∃ w : Value, ⟦ e; s ⟧ = Option.some w ∧ t = s.sub v w := by
+  constructor
+  · intro h
+    cases h with | assignment x e he
+    obtain ⟨ w, he ⟩ := he
+    grind only [Exists.choose_spec]
+  · rintro ⟨ w, heval, ht ⟩
+    rw [ht]
+    have hexists : ∃ w' : Value, some w' = e.eval? s := by
+      exists w
+      simp [*]
+    have h : hexists.choose = w := by
+      grind only [Exists.choose_spec]
+    rw [←h]
+    apply @BigStep.assignment s v e hexists
+
+@[grind =]
+theorem big_step_seq_iff (s t : State) (p₀ p₁ : Program) : (Program.seq p₀ p₁, s) ▷ t ↔ ∃ u : State, (p₀, s) ▷ u ∧ (p₁, u) ▷ t := by
+  constructor
+  · intro h
+    cases h with | @seq _ u _ d e f g
+    exists u
+  · rintro ⟨ u, ⟨ h₀, h₁ ⟩ ⟩
+    exact BigStep.seq h₀ h₁
+
+@[grind =]
+theorem big_step_cond_iff
+  (s t : State) (e : Expr) (pif pelse : Program)
+  : (Program.cond e pif pelse, s) ▷ t ↔
+  (.some (Value.bool true) = ⟦ e; s ⟧ ∧ (pif, s) ▷ t) ∨
+  (.some (Value.bool false) = ⟦ e; s ⟧ ∧ (pelse, s) ▷ t) := by
+    constructor
+    · intro h
+      cases h with
+      | cond_if hpif htrue =>
+        left
+        grind
+      | cond_else hpelse hfalse =>
+        right
+        grind
+    · intro h
+      rcases h with h | h
+      · grind [BigStep.cond_if]
+      · grind [BigStep.cond_else]
+
+@[grind =]
+theorem big_step_while_iff
+  (s t : State) (e : Expr) (p : Program)
+  : (Program.while_do e p, s) ▷ t ↔
+  (.some (Value.bool true) = ⟦ e; s ⟧ ∧ ∃ u : State, (p, s) ▷ u ∧ (Program.while_do e p, u) ▷ t) ∨
+  (.some (Value.bool false) = ⟦ e; s ⟧ ∧ s = t) := by
+    constructor
+    · intro h
+      cases h with
+      | @while_true _ u _ _ _ htrue hp hwhile => grind
+      | @while_false s _ _ hfalse => grind
+    · intro h
+      rcases h with h | h
+      · grind [BigStep.while_true]
+      · grind [BigStep.while_false]
+
+theorem big_step_while_iff'
+  (s t : State) (e : Expr) (p : Program)
+  : (Program.while_do e p, s) ▷ t ↔
+  ∃ states : List State, states[0]? = s ∧ states[states.length - 1]? = t ∧
+  ⟦ e; t ⟧ = .some (Value.bool false) ∧
+  (∀ i : Fin (states.length - 1), (p, states[i]) ▷ states[(i : Nat) + 1] ∧ ⟦ e; states[i] ⟧ = .some (Value.bool true)) := by
+    constructor
+    · sorry
+    · rintro ⟨ states, ⟨ h0, hn, hfalse, htrue ⟩ ⟩
+      revert s
+      induction states with
+      | nil => grind
+      | cons head states states_ih =>
+        intro s h0
+        simp only [Fin.getElem_fin, List.length_cons, Nat.zero_lt_succ, getElem?_pos,
+          List.getElem_cons_zero, Option.some.injEq, Nat.add_one_sub_one, Nat.lt_add_one,
+          List.getElem_cons_succ] at *
+        simp [h0] at *; clear h0
+        match states with
+        | [] => grind
+        | head' :: states =>
+          have hn' : (head' :: states)[(head' :: states).length - 1]? = some t := by
+            grind
+          specialize states_ih hn'
+          have htrue' : ∀ (i : Fin ((head' :: states).length - 1)), (p, (head' :: states)[↑i]) ▷ (head' :: states)[↑i + 1] ∧ e.eval? (head' :: states)[↑i] = some (Value.bool true) := by
+            intro i
+            specialize htrue ⟨ i + 1, by grind ⟩
+            grind
+          specialize states_ih htrue'
+          simp at states_ih
+          apply BigStep.while_true
+          · specialize htrue ⟨ 0, by grind ⟩
+            grind
+          · specialize htrue ⟨ 0, by grind ⟩
+            obtain ⟨ htrue, - ⟩ := htrue
+            simp at htrue
+            exact htrue
+          · exact states_ih
+
+theorem big_step_deterministic (p : Program) (s t u : State) (hstep : (p, s) ▷ t ∧ (p, s) ▷ u) : t = u := by
+  obtain ⟨ step₀, step₁ ⟩ := hstep
+  revert s t u
+  induction p with
+  | «skip» =>
+    grind
+  | assignment v e =>
+    grind
+  | seq p₀ p₁ hp₀ hp₁ =>
+    intro s t u hp0 hp1
+    cases hp0 with | @seq _ v _ _ _ h0 h1
+    cases hp1 with | @seq _ v' _ _ _ h0' h1'
+    specialize hp₀ s v v'
+    specialize hp₁ v t u
+    grind
+  | cond e pif pelse hif helse =>
+    grind
+  | while_do e p hp =>
+    sorry
+
+end WHILELang
